Phi_Semantics/PhiSem_Aggregate_Tuple.thy
@@ -8,9 +8,247 @@ subsection \<open>Models\<close>
 
 subsubsection \<open>Type\<close>
 
-virtual_datatype tuple_ty = \<phi>empty_ty +
+virtual_datatype tuple_ty =
   tup     :: \<open>'self list\<close>
-  array   :: \<open>'self \<times> nat\<close>
+
+debt_axiomatization T_tup :: \<open>TY list type_entry\<close>
+  where tuple_ty_ax: \<open>tuple_ty TY_CONS_OF T_tup\<close>
+
+interpretation tuple_ty TY_CONS_OF _ _ T_tup using tuple_ty_ax .
+
+(*TODO: intergrate the hidding into the automation command*)
+hide_fact tuple_ty_ax
+
+subsubsection \<open>Value\<close>
+
+virtual_datatype tuple_val =
+  V_tup     :: \<open>'self list\<close>
+
+debt_axiomatization V_tup :: \<open>VAL list value_entry\<close>
+  where tuple_val_ax: \<open>tuple_val VAL_CONS_OF V_tup\<close>
+
+interpretation tuple_val VAL_CONS_OF _ _ V_tup
+  using tuple_val_ax .
+
+hide_fact tuple_val_ax
+
+abbreviation \<open>tup \<equiv> tup.mk\<close>
+
+subsection \<open>Semantics\<close>
+
+debt_axiomatization
+        WT_tup[simp]: \<open>Well_Type (tup ts)  = { V_tup.mk vs       |vs. list_all2 (\<lambda> t v. v \<in> Well_Type t) ts vs }\<close>
+  and   zero_tup[simp]: \<open>Zero (tup Ts)     = map_option V_tup.mk (those (map Zero Ts))\<close>
+  and   V_tup_sep_disj_R[simp]: \<open>V_tup.mk l1 ## vl2 \<longleftrightarrow> (\<exists>l2. vl2 = V_tup.mk l2)\<close>
+  and   V_tup_sep_disj_L[simp]: \<open>vl1 ## V_tup.mk l2 \<longleftrightarrow> (\<exists>l1. vl1 = V_tup.mk l1)\<close>
+  and   V_tup_mult    : \<open>V_tup.mk l1 * V_tup.mk l2 = V_tup.mk (l2 @ l1)\<close>
+  and   idx_step_type_tup [eval_semantic_index] : \<open>i < length tys \<Longrightarrow> idx_step_type i (tup tys) = tys!i \<close>
+  and   valid_idx_step_tup[eval_semantic_index] : \<open>valid_idx_step (tup tys) i \<longleftrightarrow> i < length tys\<close>
+  and   idx_step_value_tup[eval_semantic_index] : \<open>idx_step_value i (V_tup.mk vs) = vs!i\<close>
+  and   idx_step_mod_value_tup : \<open>idx_step_mod_value i f (V_tup.mk vs) = V_tup.mk (vs[i := f (vs!i)])\<close>
+
+lemma V_tup_mult_cons:
+  \<open>NO_MATCH vs ([]::VAL list) \<Longrightarrow> V_tup.mk (v#vs) = V_tup.mk vs * V_tup.mk [v]\<close>
+  using V_tup_mult by simp
+
+lemma list_all_replicate:
+  \<open>list_all P (replicate n x) \<longleftrightarrow> n = 0 \<or> P x\<close>
+  by (induct n; simp; blast)
+
+lemma Valid_Type_\<tau>Tuple[simp]:
+  \<open>Valid_Type (tup Ts) \<longleftrightarrow> list_all Valid_Type Ts\<close>
+  unfolding Inhabited_def
+  by (simp; induct Ts; simp add: list_all2_Cons1)
+
+section \<open>\<phi>Type\<close>
+
+subsection \<open>Empty Tuple\<close>
+
+definition EmptyTuple :: \<open>(VAL, unit) \<phi>\<close>
+  where \<open>EmptyTuple x = { V_tup.mk [] }\<close>
+
+lemma EmptyTuple_expn[\<phi>expns]:
+  \<open>p \<in> (x \<Ztypecolon> EmptyTuple) \<longleftrightarrow> p = V_tup.mk []\<close>
+  unfolding EmptyTuple_def \<phi>Type_def by simp
+
+subsection \<open>Field\<close>
+
+definition Tuple_Field :: "(VAL, 'a) \<phi> \<Rightarrow> (VAL, 'a) \<phi>"
+  where "Tuple_Field T x = { V_tup.mk [v] |v. v \<in> T x }"
+
+syntax "_\<phi>Tuple" :: \<open>tuple_args \<Rightarrow> logic\<close> ("\<lbrace> _ \<rbrace>")
+
+translations
+  "_\<phi>Tuple (_tuple_arg X)" \<rightleftharpoons> "CONST Tuple_Field X"
+  "_\<phi>Tuple (_tuple_args y z)" \<rightleftharpoons> "CONST \<phi>Prod (_\<phi>Tuple (_tuple_arg y)) (_\<phi>Tuple z)"
+
+lemma Tuple_Field_expn[\<phi>expns]:
+  \<open>p \<in> (x \<Ztypecolon> \<lbrace> T \<rbrace>) \<longleftrightarrow> (\<exists>v. p = V_tup.mk [v] \<and> v \<in> (x \<Ztypecolon> T))\<close>
+  unfolding Tuple_Field_def \<phi>Type_def by simp
+
+lemma Tuple_Field_inhabited[elim!,\<phi>inhabitance_rule]:
+  \<open>Inhabited (x \<Ztypecolon> \<lbrace> T \<rbrace>) \<Longrightarrow> (Inhabited (x \<Ztypecolon> T) \<Longrightarrow> C) \<Longrightarrow> C\<close>
+  unfolding Inhabited_def by (simp add: \<phi>expns)
+
+lemma EmptyTuple_reduce[simp]:
+  \<open>(((),a) \<Ztypecolon> EmptyTuple \<^emph> \<lbrace> T \<rbrace>) = (a \<Ztypecolon> \<lbrace> T \<rbrace>)\<close>
+  \<open>((a,()) \<Ztypecolon> \<lbrace> T \<rbrace> \<^emph> EmptyTuple) = (a \<Ztypecolon> \<lbrace> T \<rbrace>)\<close>
+  unfolding set_eq_iff
+  apply (clarsimp; rule; clarsimp simp add: \<phi>expns V_tup_mult)
+  apply (metis V_tup_mult append_Nil)
+  apply (clarsimp; rule; clarsimp simp add: \<phi>expns V_tup_mult)
+  by (metis V_tup_mult append.right_neutral)
+
+lemma Tuple_Field_zero  [\<phi>reason 1000]:
+  \<open>\<phi>Zero ty T x \<Longrightarrow> \<phi>Zero (tup [ty]) \<lbrace> T \<rbrace> x \<close>
+  unfolding \<phi>Zero_def by (clarsimp simp add: \<phi>expns)
+
+lemma Tuple_Field_zeros [\<phi>reason 1000]:
+  \<open>\<phi>Zero ty T x
+    \<Longrightarrow> \<phi>Zero (tup tys) Ts xs
+    \<Longrightarrow> \<phi>Zero (tup (ty#tys)) (\<lbrace> T \<rbrace> \<^emph> Ts) (x,xs) \<close>
+  unfolding \<phi>Zero_def
+  apply (clarsimp simp add: \<phi>expns V_tup_mult_cons image_iff)
+  using V_tup_sep_disj_L by blast
+
+lemma Tuple_Field_semty[\<phi>reason 1000]:
+  \<open> \<phi>SemType (x \<Ztypecolon> T) TY
+\<Longrightarrow> \<phi>SemType (x \<Ztypecolon> \<lbrace> T \<rbrace>) (tup [TY])\<close>
+  unfolding \<phi>SemType_def subset_iff
+  by (clarsimp simp add: \<phi>expns)
+
+lemma Tuple_Field_semtys[\<phi>reason 1000]:
+  \<open> \<phi>SemType (x \<Ztypecolon> T) TY
+\<Longrightarrow> \<phi>SemType (xs \<Ztypecolon> Ts) (tup TYs)
+\<Longrightarrow> \<phi>SemType ((x,xs) \<Ztypecolon> (\<lbrace> T \<rbrace> \<^emph> Ts)) (tup (TY#TYs))\<close>
+  unfolding \<phi>SemType_def subset_iff
+  apply (clarsimp simp add: \<phi>expns)
+  by (metis V_tup_mult append.left_neutral append_Cons list.rel_inject(2))
+
+
+section \<open>Instruction\<close>
+
+(* definition op_cons_tuple :: "'TY list \<Rightarrow> (VAL list) proc'"
+  where "op_cons_tuple tys = (\<lambda>(vs,res).
+    let N = length tys in
+    if N \<le> length vs \<and> list_all2 (\<lambda>v t. v \<in> Well_Type t) (take N vs) tys
+    then Success (V_tup.mk (take N vs) # drop N vs, res)
+    else Fail)" *)
+
+definition op_get_tuple :: "index list \<Rightarrow> TY \<Rightarrow> (VAL, VAL) proc'"
+  where "op_get_tuple idx T = (\<lambda>v.
+    \<phi>M_getV T id v (\<lambda>v'.
+    \<phi>M_assert (valid_index T idx) \<ggreater>
+    Return (\<phi>arg (index_value idx v'))
+))"
+
+definition op_set_tuple :: "bool \<Rightarrow> TY \<Rightarrow> TY \<Rightarrow> index list \<Rightarrow> (VAL \<times> VAL, VAL) proc'"
+  where "op_set_tuple support_assigning_different_typ Tt Tv idx = 
+    \<phi>M_caseV (\<lambda>v tup.
+    \<phi>M_assert (valid_index Tt idx \<and> (support_assigning_different_typ \<or> index_type idx Tt = Tv)) \<ggreater>
+    \<phi>M_getV Tv id v (\<lambda>v'.
+    \<phi>M_getV Tt id tup (\<lambda>tup'.
+    Return (\<phi>arg (index_mod_value idx (\<lambda>_. v') tup'))
+)))"
+
+
+
+
+section \<open>Reasoning\<close>
+
+subsection \<open>Show validity of an index for a type\<close>
+
+declare [[\<phi>trace_reasoning = 1]]
+
+lemma [\<phi>reason 1200]:
+  \<open> \<s>\<i>\<m>\<p>\<r>\<e>\<m> i < length Tys
+\<Longrightarrow> Simplify eval_semantic_index Ty (Tys!i) 
+\<Longrightarrow> valid_index Ty L
+\<Longrightarrow> valid_index (tup Tys) (i#L)\<close>
+  unfolding Premise_def Simplify_def
+  by (simp add: valid_idx_step_tup idx_step_type_tup)
+
+subsection \<open>Index\<close>
+
+lemma idx_step_value_V_tup_suc:
+  \<open>idx_step_value (Suc i) (V_tup.mk (va # vs)) = idx_step_value i (V_tup.mk vs)\<close>
+  by (simp add: idx_step_value_tup)
+
+lemma idx_step_mod_value_V_tup_suc:
+  \<open>idx_step_mod_value (Suc i) g (V_tup.mk (va # vs)) = idx_step_mod_value i g (V_tup.mk vs) * V_tup.mk [va]\<close>
+  by (metis NO_MATCH_I V_tup_mult_cons idx_step_mod_value_tup list_update_code(3) nth_Cons_Suc)
+
+declare [[\<phi>trace_reasoning = 1]]
+
+lemma [\<phi>reason 1200]:
+  \<open> \<phi>Index_getter (i # idx) X Y f
+\<Longrightarrow> \<phi>Index_getter (Suc i # idx) (\<lbrace> T \<rbrace> \<^emph> X) Y (f o snd)\<close>
+  unfolding \<phi>Index_getter_def
+  by (clarsimp simp add: \<phi>expns V_tup_mult idx_step_value_V_tup_suc)
+
+lemma [\<phi>reason 1200]:
+  \<open> \<phi>Index_getter idx X Y f
+\<Longrightarrow> \<phi>Index_getter (0 # idx) \<lbrace> X \<rbrace> Y f\<close>
+  unfolding \<phi>Index_getter_def
+  by (clarsimp simp add: \<phi>expns V_tup_mult idx_step_value_tup)
+
+lemma [\<phi>reason 1200]:
+  \<open> \<phi>Index_getter idx X Y f
+\<Longrightarrow> \<phi>Index_getter (0 # idx) (\<lbrace> X \<rbrace> \<^emph> R) Y (f o fst)\<close>
+  unfolding \<phi>Index_getter_def
+  by (clarsimp simp add: \<phi>expns V_tup_mult idx_step_value_tup)
+
+lemma [\<phi>reason 1200]:
+  \<open> \<phi>Index_mapper (i # idx) X X' Y Y' f
+\<Longrightarrow> \<phi>Index_mapper (Suc i # idx) (\<lbrace> T \<rbrace> \<^emph> X) (\<lbrace> T \<rbrace> \<^emph> X') Y Y' (apsnd o f)\<close>
+  unfolding \<phi>Index_mapper_def
+  apply (clarsimp simp add: \<phi>expns V_tup_mult idx_step_mod_value_V_tup_suc)
+  by (metis V_tup_sep_disj_R idx_step_mod_value_tup)
+
+lemma [\<phi>reason 1200]:
+  \<open> \<phi>Index_mapper idx X X' Y Y' f
+\<Longrightarrow> \<phi>Index_mapper (0 # idx) \<lbrace> X \<rbrace> \<lbrace> X' \<rbrace> Y Y' f\<close>
+  unfolding \<phi>Index_mapper_def
+  by (clarsimp simp add: \<phi>expns V_tup_mult idx_step_mod_value_tup)
+
+lemma [\<phi>reason 1200]:
+  \<open> \<phi>Index_mapper idx X X' Y Y' f
+\<Longrightarrow> \<phi>Index_mapper (0 # idx) (\<lbrace> X \<rbrace> \<^emph> R) (\<lbrace> X' \<rbrace> \<^emph> R) Y Y' (apfst o f)\<close>
+  unfolding \<phi>Index_mapper_def
+  apply (clarsimp simp add: \<phi>expns V_tup_mult idx_step_mod_value_tup)
+  by (metis NO_MATCH_def V_tup_mult_cons V_tup_sep_disj_L)
+
+
+section \<open>First-level Abstraction of Instructions\<close>
+
+lemma
+  \<open> \<phi>SemType (x \<Ztypecolon> T) TY
+\<Longrightarrow> valid_index TY idx
+\<Longrightarrow> \<phi>Index_getter idx T U f
+\<Longrightarrow> \<p>\<r>\<o>\<c> op_get_tuple idx TY rv \<lbrace> x \<Ztypecolon> \<v>\<a>\<l>[rv] T \<longmapsto> f x \<Ztypecolon> \<v>\<a>\<l> U \<rbrace>\<close>
+  unfolding op_get_tuple_def \<phi>SemType_def subset_iff \<phi>Index_getter_def
+  by (cases rv; simp, rule, simp add: \<phi>expns, rule, simp add: \<phi>Mapping_expn)
+
+lemma
+  \<open> \<phi>SemType (x \<Ztypecolon> T) TY
+\<Longrightarrow> Simplify eval_semantic_index TY2 (index_type idx TY)
+\<Longrightarrow> \<phi>SemType (y \<Ztypecolon> U) TY2
+\<Longrightarrow> valid_index TY idx
+\<Longrightarrow> \<phi>Index_mapper idx T T' U' U f
+\<Longrightarrow> \<p>\<r>\<o>\<c> op_set_tuple False TY TY2 idx (ru\<^bold>, rv) \<lbrace> x \<Ztypecolon> \<v>\<a>\<l>[rv] T\<heavy_comma> y \<Ztypecolon> \<v>\<a>\<l>[ru] U \<longmapsto> f (\<lambda>_. y) x \<Ztypecolon> \<v>\<a>\<l> T' \<rbrace>\<close>
+  unfolding op_set_tuple_def \<phi>SemType_def subset_iff \<phi>Index_mapper_def Simplify_def
+  by (cases rv; cases ru; simp, rule, rule, simp add: \<phi>expns, rule, simp add: \<phi>expns,
+      rule, simp add: \<phi>Mapping_expn)
+
+lemma
+  \<open> \<phi>SemType (x \<Ztypecolon> T) TY
+\<Longrightarrow> \<phi>SemType (y \<Ztypecolon> U) TY2
+\<Longrightarrow> valid_index TY idx
+\<Longrightarrow> \<phi>Index_mapper idx T T' U' U f
+\<Longrightarrow> \<p>\<r>\<o>\<c> op_set_tuple True TY TY2 idx (ru\<^bold>, rv) \<lbrace> x \<Ztypecolon> \<v>\<a>\<l>[rv] T\<heavy_comma> y \<Ztypecolon> \<v>\<a>\<l>[ru] U \<longmapsto> f (\<lambda>_. y) x \<Ztypecolon> \<v>\<a>\<l> T' \<rbrace>\<close>
+  unfolding op_set_tuple_def \<phi>SemType_def subset_iff \<phi>Index_mapper_def Simplify_def
+  by (cases rv; cases ru; simp, rule, rule, simp add: \<phi>expns, rule, simp add: \<phi>expns,
+      rule, simp add: \<phi>Mapping_expn)
 
 
 end
